theories/cancellation/InlineElim.v
@@ -1,12 +1,12 @@
-From iris.proofmode Require Import proofmode.
 Require Import Common.
+From iris.proofmode Require Import proofmode.
 Require Import SModTr SMod HMod ITactics.
 Require Import ISim ISimInit CtxRefine CtxRefineFacts ClosedAdequacy.
 Require Import HModInline.
 
 Set Implicit Arguments.
 
-Lemma cancel_call_rev `{Σ: GRA} md P
+Lemma inline_elim `{Σ: GRA} md P
 :
   refines (md, P) (HModInline.inline md, P).
 Proof. 
@@ -17,28 +17,33 @@ Proof.
   destruct (alist_find fn (HMod.fnsems md)) eqn:FINDT; ss.
     
   inv FIND.
-     (* rename p into ft. *)
-     esplits; eauto.
-    { rewrite alist_find_map_snd. rewrite FINDT. ss. }
-  ii. subst. destruct fs.
+  esplits; eauto.
+  { rewrite alist_find_map_snd. rewrite FINDT. ss. }
+  ii. subst. destruct fs as [[msk sc] f].
   assert(SCP := md.(HMod.well_scoped_fns)).
   specialize (SCP fn). rewrite/fnsems_scopes FINDT in SCP.
-  remember (HMod.scopes md) as scopeS. i.
-  rename l into scopeT. 
-  unfold wrap_elimI. s. unfold HModTr.sandbox_body, inline_hp_fun. s.
+  remember (HMod.scopes md) as scopes. i.
+  unfold wrap_elimI, HModTr.sandbox_body, inline_hp_fbody. s.
+  unfold HModTr.sandbox_body, inline_hp_fun. s.
   generalize false at 1 as ps.
   generalize false at 1 as pt. intros pt ps.
-  generalize (i y) as it. clear IN fn FINDT i y NODD NODS.
+  generalize (f y) as it.
+  assert (IMPSC: exists fn f, alist_find fn (HMod.fnsems md) = Some (msk,sc,f)).
+  { eauto. }
+  clear IN y NODD NODS FINDT fn f. i.
+
+  revert SCP.
+  combine_quant IMPSC.
+  combine_quant msk.
+  combine_quant sc.
+  combine_quant it.
   combine_quant st_tgt.
   combine_quant st_src.
-  combine_quant SCP.
-  combine_quant scopeT.
   combine_quant pt.
   combine_quant ps.
   combine_quant nths.
   eapply isim_coind. i.
-
-  destruct a as [nths [ps [pt [scopeT [SCP [st_src [st_tgt it]]]]]]]. s.
+  destruct a as [nths [ps [pt [st_src [st_tgt [it [sc [msk [IMPSC SCP]]]]]]]]]. s.
 
   iIntros "(Ist & #CIH)".
 
@@ -49,12 +54,12 @@ Proof.
   - rewrite SBRed.bind SBRed.ag HIRed.bind_ag. steps_r. force_l. iFrame. steps_l. by_coind "CIH". eauto.
   - destruct c.
     {
-      rewrite SBRed.bind SBRed.call.
+      rewrite SBRed.bind SBRed.call. des_ifs; cycle 1.
+      { steps_l. ss. }
       rewrite HIRed.call. steps_r.
-      destruct (alist_find fn (HMod.fnsems md)) eqn:FIND; cycle 1.
+      destruct (alist_find fn0 (HMod.fnsems md)) eqn:FIND; cycle 1.
       { s. iApply isim_call_none; ss.
-        { rewrite alist_find_map_snd FIND. ss. }
-        unfold triggerUB. ired. rewrite HIRed.bind_core. steps_l. ss.
+        rewrite alist_find_map_snd FIND. ss.
       }
       destruct p. iApply isim_inline_src.
       { rewrite alist_find_map_snd FIND. ss. }
@@ -68,9 +73,9 @@ Proof.
       rewrite HIRed.tau. steps_l. steps_r. ired.
       by_coind "CIH". auto.
     }
-    {
-      rewrite SBRed.bind SBRed.spawn.
-      rewrite HIRed.bind_spawn SBRed.bind SBRed.spawn.
+    { rewrite SBRed.bind SBRed.spawn. des_ifs; cycle 1.
+      { steps_l. ss. }
+      rewrite HIRed.bind_spawn SBRed.bind SBRed.spawn. s.
       iApply isim_spawn. steps_r. by_coind "CIH". auto.
     }
     { rewrite !SBRed.bind SBRed.yield HIRed.bind_yield SBRed.bind SBRed.yield.
@@ -107,9 +112,9 @@ Proof.
     + steps_l. force_r. steps_r. instantiate (1:= q). by_coind "CIH". auto.
     + step. steps_l. steps_r. by_coind "CIH". auto.
   Unshelve. all: try refl; eauto.
+  { destruct p. eauto. }
   {
-    assert(SCP0 := md.(HMod.well_scoped_fns) fn).
+    assert(SCP0 := md.(HMod.well_scoped_fns) fn0).
     rewrite/fnsems_scopes FIND in SCP0. eauto.
   }
 (*SLOW*)Qed.
-
